@prefix : <http://www.semanticweb.org/juan/ontologies/2024/3/satisfaccion-aerolineas/> .
@prefix owl: <http://www.w3.org/2002/07/owl#> .
@prefix rdf: <http://www.w3.org/1999/02/22-rdf-syntax-ns#> .
@prefix xml: <http://www.w3.org/XML/1998/namespace> .
@prefix xsd: <http://www.w3.org/2001/XMLSchema#> .
@prefix rdfs: <http://www.w3.org/2000/01/rdf-schema#> .
@base <http://www.semanticweb.org/juan/ontologies/2024/3/satisfaccion-aerolineas/> .

<http://www.semanticweb.org/juan/ontologies/2024/3/satisfaccion-aerolineas> rdf:type owl:Ontology ;
                                                                             rdfs:comment "Author: Juan Eiros Zamora" .

#################################################################
#    Annotation properties
#################################################################

###  http://www.w3.org/2000/01/rdf-schema#sameAs
rdfs:sameAs rdf:type owl:AnnotationProperty .


#################################################################
#    Object Properties
#################################################################

###  http://www.semanticweb.org/juan/ontologies/2024/3/satisfaccion-aerolineas/author
:author rdf:type owl:ObjectProperty ;
        owl:inverseOf :submits ;
        rdfs:domain :Survey ;
        rdfs:range :Passenger ;
        rdfs:comment "The individual who writes and submits a survey or review about a flight experience." ;
        rdfs:label "Author" .


###  http://www.semanticweb.org/juan/ontologies/2024/3/satisfaccion-aerolineas/hasSeatType
:hasSeatType rdf:type owl:ObjectProperty ,
                      owl:FunctionalProperty ;
             rdfs:domain :Flight ;
             rdfs:range :Seat ;
             rdfs:comment "Indicates the type of seat that a passenger has booked or been assigned on a flight." ;
             rdfs:label "Has Seat Type" .


###  http://www.semanticweb.org/juan/ontologies/2024/3/satisfaccion-aerolineas/operatedBy
:operatedBy rdf:type owl:ObjectProperty ;
            owl:inverseOf :operates ;
            rdf:type owl:FunctionalProperty ;
            rdfs:domain :Flight ;
            rdfs:range :Airline ;
            rdfs:comment "Shows the airline that operates a specific flight." ;
            rdfs:label "Operated By" .


###  http://www.semanticweb.org/juan/ontologies/2024/3/satisfaccion-aerolineas/operates
:operates rdf:type owl:ObjectProperty ;
          rdfs:domain :Airline ;
          rdfs:range :Flight ;
          rdfs:comment "Links an airline to the flight that it operates." ;
          rdfs:label "Operates" .


###  http://www.semanticweb.org/juan/ontologies/2024/3/satisfaccion-aerolineas/reviewedIn
:reviewedIn rdf:type owl:ObjectProperty ;
            rdfs:domain :Flight ;
            rdfs:range :Survey ;
            rdfs:comment "Connects a flight to the survey in which it has been reviewed." ;
            rdfs:label "Reviewed In" .


###  http://www.semanticweb.org/juan/ontologies/2024/3/satisfaccion-aerolineas/submits
:submits rdf:type owl:ObjectProperty ;
         rdfs:domain :Passenger ;
         rdfs:range :Survey ;
         rdfs:comment "Represents the action of a passenger submitting a survey or review about their flight experience." ;
         rdfs:label "Submits" .


#################################################################
#    Data properties
#################################################################

###  http://www.semanticweb.org/juan/ontologies/2024/3/satisfaccion-aerolineas/aircraft
:aircraft rdf:type owl:DatatypeProperty ;
          rdfs:domain :Flight ;
          rdfs:range xsd:string ;
          rdfs:comment "Identifies the aircraft used for a specific flight." ;
          rdfs:label "Aircraft" ;
          rdfs:sameAs "https://dbpedia.org/page/Aircraft" .


###  http://www.semanticweb.org/juan/ontologies/2024/3/satisfaccion-aerolineas/body
:body rdf:type owl:DatatypeProperty ;
      rdfs:domain :Survey ;
      rdfs:range xsd:string ;
      rdfs:comment "Contains the main text of a passenger's review detailing their flight experience." ;
      rdfs:label "Review Body" .


###  http://www.semanticweb.org/juan/ontologies/2024/3/satisfaccion-aerolineas/country
:country rdf:type owl:DatatypeProperty ;
         rdfs:domain :Airline ;
         rdfs:range xsd:string ;
         rdfs:comment "Denotes the country related to a specific context, such as airline registration or passenger nationality." ;
         rdfs:label "Country" ;
         rdfs:sameAs "https://dbpedia.org/page/Country" .


###  http://www.semanticweb.org/juan/ontologies/2024/3/satisfaccion-aerolineas/countryOfOrigin
:countryOfOrigin rdf:type owl:DatatypeProperty ;
                 rdfs:domain :Passenger ;
                 rdfs:range xsd:string ;
                 rdfs:comment "Indicates the country where a passenger or crew member originates from." ;
                 rdfs:label "Country of Origin" .


###  http://www.semanticweb.org/juan/ontologies/2024/3/satisfaccion-aerolineas/datePublished
:datePublished rdf:type owl:DatatypeProperty ;
               rdfs:domain :Survey ;
               rdfs:range xsd:dateTime ;
               rdfs:comment "The date when a review or survey was published." ;
               rdfs:label "Date Published" .


###  http://www.semanticweb.org/juan/ontologies/2024/3/satisfaccion-aerolineas/destination
:destination rdf:type owl:DatatypeProperty ;
             rdfs:domain :Flight ;
             rdfs:range xsd:string ;
             rdfs:comment "The final arrival airport of a flight." ;
             rdfs:label "Destination" .


###  http://www.semanticweb.org/juan/ontologies/2024/3/satisfaccion-aerolineas/flightDate
:flightDate rdf:type owl:DatatypeProperty ;
            rdfs:domain :Flight ;
            rdfs:range xsd:dateTime ;
            rdfs:comment "The date when a flight took place." ;
            rdfs:label "Flight Date" ;
            rdfs:sameAs "https://dbpedia.org/page/Calendar_date" .


###  http://www.semanticweb.org/juan/ontologies/2024/3/satisfaccion-aerolineas/name
:name rdf:type owl:DatatypeProperty ;
      rdfs:domain :Airline ,
                  :Passenger ;
      rdfs:range xsd:string ;
      rdfs:comment "A person's full name or an entity's official name." ;
      rdfs:label "Name" .


###  http://www.semanticweb.org/juan/ontologies/2024/3/satisfaccion-aerolineas/origin
:origin rdf:type owl:DatatypeProperty ;
        rdfs:domain :Flight ;
        rdfs:range xsd:string ;
        rdfs:comment "The starting location of a flight." ;
        rdfs:label "Origin" .


###  http://www.semanticweb.org/juan/ontologies/2024/3/satisfaccion-aerolineas/rating
:rating rdf:type owl:DatatypeProperty ;
        rdfs:domain :Survey ;
        rdfs:range xsd:double ;
        rdfs:comment "A score given by a passenger to rate their flight experience, typically on a scale." ;
        rdfs:label "Rating" .


###  http://www.semanticweb.org/juan/ontologies/2024/3/satisfaccion-aerolineas/recommended
:recommended rdf:type owl:DatatypeProperty ;
             rdfs:domain :Survey ;
             rdfs:range xsd:boolean ;
             rdfs:comment "Indicates whether a passenger recommends the airline after their experience." ;
             rdfs:label "Recommended" .


###  http://www.semanticweb.org/juan/ontologies/2024/3/satisfaccion-aerolineas/title
:title rdf:type owl:DatatypeProperty ;
       rdfs:domain :Survey ;
       rdfs:range xsd:string ;
       rdfs:comment "The title of a review or survey entry." ;
       rdfs:label "Title" .


#################################################################
#    Classes
#################################################################

###  http://www.semanticweb.org/juan/ontologies/2024/3/satisfaccion-aerolineas/Airline
:Airline rdf:type owl:Class ;
         rdfs:comment "An organization that provides air transport services for traveling passengers." ;
         rdfs:label "Airline" .


###  http://www.semanticweb.org/juan/ontologies/2024/3/satisfaccion-aerolineas/BusinessClass
:BusinessClass rdf:type owl:Class ;
               rdfs:subClassOf :Seat ;
               rdfs:comment "A high-quality seat class on a flight that offers additional space, comfort, and service. It is the most expensive kind of seat, suited for people that travel for work purposes." ;
               rdfs:label "Business Class Seat" .


###  http://www.semanticweb.org/juan/ontologies/2024/3/satisfaccion-aerolineas/CabinCrew
:CabinCrew rdf:type owl:Class ;
           rdfs:subClassOf :CrewMember ;
           rdfs:comment "A crew member who is responsible for the safety and comfort of passengers during a flight." ;
           rdfs:label "Cabin Crew" .


###  http://www.semanticweb.org/juan/ontologies/2024/3/satisfaccion-aerolineas/CrewMember
:CrewMember rdf:type owl:Class ;
            rdfs:comment "An individual who is a member of the flight crew, responsible for the operation of the aircraft and service during the flight." ;
            rdfs:label "Crew Member" .


###  http://www.semanticweb.org/juan/ontologies/2024/3/satisfaccion-aerolineas/EconomyClass
:EconomyClass rdf:type owl:Class ;
              rdfs:subClassOf :Seat ;
              rdfs:comment "A standard seat class on a flight offering basic services with an emphasis on affordability." ;
              rdfs:label "Economy Class Seat" .


###  http://www.semanticweb.org/juan/ontologies/2024/3/satisfaccion-aerolineas/EntertainmentSystem
:EntertainmentSystem rdf:type owl:Class ;
                     rdfs:subClassOf :FlightServices ;
                     rdfs:comment "An electronic system provided to passengers during a flight for leisure, such as movies, music, or games." ;
                     rdfs:label "Entertainment System" .


###  http://www.semanticweb.org/juan/ontologies/2024/3/satisfaccion-aerolineas/Flight
:Flight rdf:type owl:Class ;
        rdfs:comment "A scheduled journey of an aircraft from one airport to another." ;
        rdfs:label "Flight" .


###  http://www.semanticweb.org/juan/ontologies/2024/3/satisfaccion-aerolineas/FlightServices
:FlightServices rdf:type owl:Class ;
                rdfs:comment "A series of ammenities and other various services provided to passengers of a flight." ;
                rdfs:label "Flight Services" .


###  http://www.semanticweb.org/juan/ontologies/2024/3/satisfaccion-aerolineas/Internet
:Internet rdf:type owl:Class ;
          rdfs:subClassOf :FlightServices ;
          rdfs:comment "The ability to connect passenger's electronic devices to the public Internet." ;
          rdfs:label "Internet" .


###  http://www.semanticweb.org/juan/ontologies/2024/3/satisfaccion-aerolineas/LongHaul
:LongHaul rdf:type owl:Class ;
          rdfs:subClassOf :Flight ;
          rdfs:comment "A flight that covers a great distance and typically has a duration of six hours or more." ;
          rdfs:label "Long Haul Flight" .


###  http://www.semanticweb.org/juan/ontologies/2024/3/satisfaccion-aerolineas/Luggage
:Luggage rdf:type owl:Class ;
         rdfs:comment "Personal belongings of passengers transported in the aircraft's hold or cabin." ;
         rdfs:label "Luggage" .


###  http://www.semanticweb.org/juan/ontologies/2024/3/satisfaccion-aerolineas/MealService
:MealService rdf:type owl:Class ;
             rdfs:subClassOf :FlightServices ;
             rdfs:comment "A service provided on a flight that includes the offering of meals and beverages to passengers." ;
             rdfs:label "Meal Service" .


###  http://www.semanticweb.org/juan/ontologies/2024/3/satisfaccion-aerolineas/Passenger
:Passenger rdf:type owl:Class ;
           rdfs:comment "An individual who travels in an aircraft." ;
           rdfs:label "Passenger" .


###  http://www.semanticweb.org/juan/ontologies/2024/3/satisfaccion-aerolineas/Pilot
:Pilot rdf:type owl:Class ;
       rdfs:subClassOf :CrewMember ;
       rdfs:comment "A crew member who is qualified to operate the aircraft and is responsible for navigating the flight." ;
       rdfs:label "Pilot" .


###  http://www.semanticweb.org/juan/ontologies/2024/3/satisfaccion-aerolineas/QatarAirways
:QatarAirways rdf:type owl:Class ;
              rdfs:subClassOf :Airline ;
              rdfs:comment "The state-owned flag carrier of Qatar, known for its high-quality service and global flight network." ;
              rdfs:label "Qatar Airways" .


###  http://www.semanticweb.org/juan/ontologies/2024/3/satisfaccion-aerolineas/QatarAirwaysSurvey
:QatarAirwaysSurvey rdf:type owl:Class ;
                    rdfs:subClassOf :Survey ;
                    rdfs:comment "A passenger's survey response specifically related to a Qatar Airways flight experience." ;
                    rdfs:label "Qatar Airways Survey" .


###  http://www.semanticweb.org/juan/ontologies/2024/3/satisfaccion-aerolineas/Ryanair
:Ryanair rdf:type owl:Class ;
         rdfs:subClassOf :Airline ;
         rdfs:comment "An Irish low-cost carrier with a wide network of short-haul and medium-haul flights across Europe and North Africa." ;
         rdfs:label "Ryanair" .


###  http://www.semanticweb.org/juan/ontologies/2024/3/satisfaccion-aerolineas/RyanairSurvey
:RyanairSurvey rdf:type owl:Class ;
               rdfs:subClassOf :Survey ;
               rdfs:comment "A passenger's survey response specifically related to a Ryanair flight experience." ;
               rdfs:label "Ryanair Survey" .


###  http://www.semanticweb.org/juan/ontologies/2024/3/satisfaccion-aerolineas/Seat
:Seat rdf:type owl:Class ;
      rdfs:comment "A place for a passenger to sit on a flight, can be classified into various categories based on comfort and services." ;
      rdfs:label "Seat" .


###  http://www.semanticweb.org/juan/ontologies/2024/3/satisfaccion-aerolineas/ShortHaul
:ShortHaul rdf:type owl:Class ;
           rdfs:subClassOf :Flight ;
           rdfs:comment "A flight that covers a short distance, typically within the same continent and lasting less than six hours." ;
           rdfs:label "Short Haul Flight" .


###  http://www.semanticweb.org/juan/ontologies/2024/3/satisfaccion-aerolineas/Survey
:Survey rdf:type owl:Class ;
        rdfs:comment "An evaluation or review given by a passenger that reflects their experience and satisfaction with a flight." ;
        rdfs:label "Survey" .


#################################################################
#    Individuals
#################################################################

###  http://www.semanticweb.org/juan/ontologies/2024/3/satisfaccion-aerolineas/FlightQR001
:FlightQR001 rdf:type owl:NamedIndividual ,
                      :LongHaul ;
             :destination "LHR" ;
             :origin "DOH" ;
             rdfs:label "Flight QR001" .


###  http://www.semanticweb.org/juan/ontologies/2024/3/satisfaccion-aerolineas/JohnDoePassenger
:JohnDoePassenger rdf:type owl:NamedIndividual ,
                           :Passenger ;
                  :name "John Doe" ;
                  rdfs:label "John Doe" .


###  http://www.semanticweb.org/juan/ontologies/2024/3/satisfaccion-aerolineas/Qatar_Airways
:Qatar_Airways rdf:type owl:NamedIndividual ,
                        :QatarAirways ;
               :country "Qatar" ;
               :name "Qatar Airways" ;
               rdfs:label "Qatar Airways" .


###  http://www.semanticweb.org/juan/ontologies/2024/3/satisfaccion-aerolineas/Seat1A
:Seat1A rdf:type owl:NamedIndividual ,
                 :BusinessClass ;
        :aircraft "Boeing" ;
        rdfs:label "Seat 1A" .


###  http://www.semanticweb.org/juan/ontologies/2024/3/satisfaccion-aerolineas/Survey001
:Survey001 rdf:type owl:NamedIndividual ,
                    :QatarAirwaysSurvey .


###  Generated by the OWL API (version 4.5.26.2023-07-17T20:34:13Z) https://github.com/owlcs/owlapi
